io/case-studies/Compiler.Model1.Examples.fst
@@ -12,14 +12,14 @@ open Compiler.Model1
 type source_arrow (mst:mst) (arg:Type u#a) (res:Type u#b) (pre:arg -> trace -> Type0) (post:arg -> trace -> resexn res -> trace -> Type0) (fl:erased tflag) =
   x:arg -> MIO (resexn res) mst fl (pre x) (post x)
 
-type c1typ (#arg:Type u#a) (#res:Type u#b) (pre:arg -> trace -> Type0) (post:arg -> trace -> resexn res -> trace -> Type0) (pi:policy_spec) =
-  squash (forall x h lt. pre x h /\ enforced_locally pi h lt ==> post x h (Inr Contract_failure) lt)
+type c1typ (#arg:Type u#a) (#res:Type u#b) (pre:arg -> trace -> Type0) (post:arg -> trace -> resexn res -> trace -> Type0) (sgm:policy_spec) =
+  squash (forall x h lt. pre x h /\ enforced_locally sgm h lt ==> post x h (Inr Contract_failure) lt)
   
-type c2typ (#arg:Type u#a) (#res:Type u#b) (pre:arg -> trace -> Type0) (post:arg -> trace -> resexn res -> trace -> Type0) (pi:policy_spec) (#mst:mst) (dc:dc_typ mst #arg #(resexn res)) =
-  squash (forall s0 s1 x h r lt . s0 `mst.models` h /\ s1 `mst.models` (apply_changes h lt) /\ pre x h /\ enforced_locally pi h lt /\ dc x s0 r s1 ==> post x h r lt)
+type c2typ (#arg:Type u#a) (#res:Type u#b) (pre:arg -> trace -> Type0) (post:arg -> trace -> resexn res -> trace -> Type0) (sgm:policy_spec) (#mst:mst) (dc:dc_typ mst #arg #(resexn res)) =
+  squash (forall s0 s1 x h r lt . s0 `mst.models` h /\ s1 `mst.models` (apply_changes h lt) /\ pre x h /\ enforced_locally sgm h lt /\ dc x s0 r s1 ==> post x h r lt)
 
-type stronger_pis (pi1:policy_spec) (pi2:policy_spec) =
-  squash (forall h lt. enforced_locally pi1 h lt ==> enforced_locally pi2 h lt)
+type stronger_sgms (sgm1:policy_spec) (sgm2:policy_spec) =
+  squash (forall h lt. enforced_locally sgm1 h lt ==> enforced_locally sgm2 h lt)
   
 #push-options "--compat_pre_core 1"
 
@@ -37,14 +37,14 @@ let mst1 : mst = {
 
 type test1_ct = source_arrow mst1 unit file_descr test1_pre test1_post
 
-let test1_pi : policy_spec = 
+let test1_sgm : policy_spec = 
   fun h c cmd arg -> 
     Ctx? c /\
     (match cmd with 
     | Openfile -> (arg <> "/etc/passwd")
     | _ -> True)
 
-let test1_phi : policy mst1 test1_pi =
+let test1_pi : policy mst1 test1_sgm =
   fun h cmd arg -> 
     match cmd, arg with 
     | Openfile, s ->
@@ -63,10 +63,10 @@ let test1_ct_rcs : tree (pck_dc mst1) =
     Leaf 
     Leaf
 
-val test1_c1post : c1typ test1_pre test1_post test1_pi 
+val test1_c1post : c1typ test1_pre test1_post test1_sgm 
 let test1_c1post = 
   let rec aux (h:trace) (lt:trace) : Lemma
-    (requires (enforced_locally test1_pi h lt))
+    (requires (enforced_locally test1_sgm h lt))
     (ensures (test1_post () h (Inr Contract_failure) lt))
     (decreases lt) = (
     match lt with
@@ -74,41 +74,41 @@ let test1_c1post =
     | e :: tail -> aux (e::h) tail) in
   Classical.forall_intro_2 (Classical.move_requires_2 aux)
 
-let rec enforced_locally_test1_pi_nopass h lt fd :
+let rec enforced_locally_test1_sgm_nopass h lt fd :
   Lemma
-    (requires enforced_locally test1_pi h lt)
+    (requires enforced_locally test1_sgm h lt)
     (ensures ~((EOpenfile Ctx "/etc/passwd" fd) `memP` lt))
     (decreases lt)
 = match lt with
   | EOpenfile Ctx "/etc/passwd" fd' :: tl ->
     if fd = fd'
     then ()
-    else enforced_locally_test1_pi_nopass (EOpenfile Ctx "/etc/passwd" fd' :: h) tl fd
+    else enforced_locally_test1_sgm_nopass (EOpenfile Ctx "/etc/passwd" fd' :: h) tl fd
   | e :: tl ->
-    enforced_locally_test1_pi_nopass (e :: h) tl fd
+    enforced_locally_test1_sgm_nopass (e :: h) tl fd
   | [] -> ()
 
-val test1_c2post : c2typ test1_pre test1_post test1_pi test1_ct_rc
+val test1_c2post : c2typ test1_pre test1_post test1_sgm test1_ct_rc
 let test1_c2post =
-  introduce forall s0 s1 x h r lt . s0 `mst1.models` h /\ s1 `mst1.models` (apply_changes h lt) /\ test1_pre x h /\ enforced_locally test1_pi h lt /\ test1_ct_rc x s0 r s1 ==> test1_post x h r lt
+  introduce forall s0 s1 x h r lt . s0 `mst1.models` h /\ s1 `mst1.models` (apply_changes h lt) /\ test1_pre x h /\ enforced_locally test1_sgm h lt /\ test1_ct_rc x s0 r s1 ==> test1_post x h r lt
   with begin
-    introduce s0 `mst1.models` h /\ s1 `mst1.models` (apply_changes h lt) /\ test1_pre x h /\ enforced_locally test1_pi h lt /\ test1_ct_rc x s0 r s1 ==> test1_post x h r lt
+    introduce s0 `mst1.models` h /\ s1 `mst1.models` (apply_changes h lt) /\ test1_pre x h /\ enforced_locally test1_sgm h lt /\ test1_ct_rc x s0 r s1 ==> test1_post x h r lt
     with _. begin
       introduce forall fd'. ~((EOpenfile Ctx "/etc/passwd" fd') `memP` lt)
-      with enforced_locally_test1_pi_nopass h lt fd'
+      with enforced_locally_test1_sgm_nopass h lt fd'
     end
   end
 
 #set-options "--print_implicits"
 
-let test1_ct_importable (fl:erased tflag) : safe_importable (test1_ct fl) fl test1_pi mst1 test1_ct_rcs =
+let test1_ct_importable (fl:erased tflag) : safe_importable (test1_ct fl) fl test1_sgm mst1 test1_ct_rcs =
   safe_importable_arrow_pre_post_args_res _ _ test1_c1post test1_c2post #exportable_unit #importable_file_descr
 
-val test1_stronger_pis : stronger_pis test1_pi test1_pi
-let test1_stronger_pis = 
+val test1_stronger_sgms : stronger_sgms test1_sgm test1_sgm
+let test1_stronger_sgms = 
   let rec aux (h:trace) (lt:trace) : Lemma
-    (requires (enforced_locally test1_pi h lt))
-    (ensures (enforced_locally test1_pi h lt))
+    (requires (enforced_locally test1_sgm h lt))
+    (ensures (enforced_locally test1_sgm h lt))
     (decreases lt) = (match lt with
     | [] -> ()
     | e :: tail -> aux (e::h) tail) in 
@@ -117,7 +117,7 @@ let test1_stronger_pis =
 [@@ (postprocess_with (fun () -> norm [delta_only [`%test1_ct; `%source_arrow; `%test1_ct_importable]]; trefl ()))]
 let test1 : src_interface = {
   mst = mst1;
-  pi = test1_pi; phi = test1_phi;
+  sgm = test1_sgm; pi = test1_pi;
 
   ct = test1_ct;
   ct_dcs = test1_ct_rcs;
@@ -137,7 +137,7 @@ let test1_ctx #fl sec_io eff_rcs () : MIO (resexn file_descr) mst1 fl (fun _ -> 
   sec_io Openfile "/etc/passwd"
 
 val test1_ctx_t : ctx_tgt (comp_int_src_tgt test1)
-let test1_ctx_t #fl sec_io () : MIOpi (resexn file_descr) fl test1_pi mst1 =
+let test1_ctx_t #fl sec_io () : MIOpi (resexn file_descr) fl test1_sgm mst1 =
   sec_io Openfile "/etc/passwd"
 
 
@@ -147,8 +147,8 @@ let mst2 : mst = {
   models = (fun s h -> forall fd. memP fd s <==> is_open fd h);
 }
 
-let test2_pi : policy_spec = (fun _ _ _ _ -> true)
-let test2_phi : policy mst2 test2_pi = (fun _ _ _ -> true)
+let test2_sgm : policy_spec = (fun _ _ _ _ -> true)
+let test2_pi : policy mst2 test2_sgm = (fun _ _ _ -> true)
 
 let test2_cb (fl:erased tflag) = (fd:file_descr -> MIO (resexn unit) mst2 fl (fun h -> is_open fd h) (fun _ _ lt -> lt == []))
 let test2_post = (fun _ h (rfd:resexn file_descr) lt -> Inl? rfd ==> is_open (Inl?.v rfd) (rev lt @ h))
@@ -163,15 +163,15 @@ let test2_rcs : tree (pck_dc mst2) =
      (Node (| file_descr, unit, (fun fd s0 _ _ -> fd `List.mem` s0) |) Leaf Leaf)
      Leaf
   
-val test2_c1post (a:Type) : c1typ #a #file_descr (fun _ _ -> True) test2_post test2_pi
+val test2_c1post (a:Type) : c1typ #a #file_descr (fun _ _ -> True) test2_post test2_sgm
 let test2_c1post a = ()
 
 
-val test2_c2post (a:Type) : squash (forall s0 s1 (x:a) h r lt . s0 `mst2.models` h /\ s1 `mst2.models` (apply_changes h lt) /\ enforced_locally test2_pi h lt /\ test2_rc () s0 r s1 ==> test2_post x h r lt)
+val test2_c2post (a:Type) : squash (forall s0 s1 (x:a) h r lt . s0 `mst2.models` h /\ s1 `mst2.models` (apply_changes h lt) /\ enforced_locally test2_sgm h lt /\ test2_rc () s0 r s1 ==> test2_post x h r lt)
 let test2_c2post a = ()
 
-let test2_ct_importable (fl:erased tflag) : safe_importable (test2_ct fl) fl test2_pi mst2 test2_rcs = 
-  let exportable_cb = exportable_arrow_pre_post_args file_descr unit #fl #test2_pi #mst2 #(left test2_rcs) (fun fd h -> is_open fd h) (fun fd _ _ lt -> lt == []) in
+let test2_ct_importable (fl:erased tflag) : safe_importable (test2_ct fl) fl test2_sgm mst2 test2_rcs = 
+  let exportable_cb = exportable_arrow_pre_post_args file_descr unit #fl #test2_sgm #mst2 #(left test2_rcs) (fun fd h -> is_open fd h) (fun fd _ _ lt -> lt == []) in
   safe_importable_arrow_pre_post_res
     (fun _ _ -> True)  (** pre **)
     test2_post       (** post **)
@@ -183,7 +183,7 @@ let test2_ct_importable (fl:erased tflag) : safe_importable (test2_ct fl) fl tes
 [@@ (postprocess_with (fun () -> norm [delta_only [`%test2_ct; `%test2_cb;`%test2_ct_importable]]; trefl ()))]
 let test2 : src_interface = {
   mst = mst2;
-  pi = test2_pi; phi = test2_phi; 
+  sgm = test2_sgm; pi = test2_pi; 
   ct = test2_ct; ct_dcs = test2_rcs; ct_importable = test2_ct_importable; 
   psi = (fun _ _ _ -> True);
 }
@@ -203,7 +203,7 @@ let test2_ctx #fl sec_io eff_rcs cb : MIO (resexn file_descr) mst2 fl (fun _ -> 
   | _ -> rfd
 
 val test2_ctx_t : ctx_tgt (comp_int_src_tgt test2)
-let test2_ctx_t #fl sec_io cb : MIOpi (resexn file_descr) fl (comp_int_src_tgt test2).pi mst2 = 
+let test2_ctx_t #fl sec_io cb : MIOpi (resexn file_descr) fl (comp_int_src_tgt test2).sgm mst2 = 
   let rfd = sec_io Openfile "/etc/passwd" in
   match rfd with
   | Inl fd -> begin
@@ -219,8 +219,8 @@ let mst3 : mst = {
   models = (fun s h -> forall fd. memP fd s <==> is_open fd h);
 }
 
-let test3_pi : policy_spec = (fun _ _ _ _ -> true)
-let test3_phi : policy mst3 test3_pi = (fun _ _ _ -> true)
+let test3_sgm : policy_spec = (fun _ _ _ _ -> true)
+let test3_pi : policy mst3 test3_sgm = (fun _ _ _ -> true)
 
 let test3_cb (fl:erased tflag) = (fd:file_descr -> MIO (resexn unit) mst3 fl (fun h -> True) (fun _ _ lt -> True))
 let test3_post #a = (fun (x:file_descr) h (r:a) lt -> True)
@@ -231,11 +231,11 @@ let test3_rcs : tree (pck_dc mst3) =
      Leaf
      (Node (| file_descr, resexn unit, (fun _ _ _ _ -> true) |) Leaf Leaf)
 
-let test3_cb_importable (fl:erased tflag) : safe_importable (test3_cb fl) fl test3_pi mst3 (right test3_rcs) = 
+let test3_cb_importable (fl:erased tflag) : safe_importable (test3_cb fl) fl test3_sgm mst3 (right test3_rcs) = 
   safe_importable_arrow_pre_post_args_res
     #file_descr #unit
     #fl
-    #test3_pi
+    #test3_sgm
     #mst3
     #(right test3_rcs)
     (fun fd h -> True)
@@ -245,16 +245,16 @@ let test3_cb_importable (fl:erased tflag) : safe_importable (test3_cb fl) fl tes
     #exportable_file_descr
     #importable_unit
   
-val test3_c1post (a:Type) : c1typ #file_descr #a (fun _ _ -> True) test3_post test3_pi 
+val test3_c1post (a:Type) : c1typ #file_descr #a (fun _ _ -> True) test3_post test3_sgm 
 let test3_c1post a = ()
   
 val test3_c2post (a:Type) : 
-  squash (forall s0 s1 x h r lt . s0 `mst3.models` h /\ s1 `mst3.models` (apply_changes h lt) /\ enforced_locally test3_pi h lt /\ (root test3_rcs)._3 x s0 r s1 ==> test3_post x h r lt)
+  squash (forall s0 s1 x h r lt . s0 `mst3.models` h /\ s1 `mst3.models` (apply_changes h lt) /\ enforced_locally test3_sgm h lt /\ (root test3_rcs)._3 x s0 r s1 ==> test3_post x h r lt)
 let test3_c2post a = ()
 
-let test3_ct_importable (fl:erased tflag) : safe_importable (test3_ct fl) fl test3_pi mst3 test3_rcs = 
+let test3_ct_importable (fl:erased tflag) : safe_importable (test3_ct fl) fl test3_sgm mst3 test3_rcs = 
   safe_importable_arrow_pre_post_args
-    #file_descr #(test3_cb fl) #fl #test3_pi #mst3 #test3_rcs
+    #file_descr #(test3_cb fl) #fl #test3_sgm #mst3 #test3_rcs
     (fun _ _ -> True)  (** pre **)
     test3_post       (** post **)
     (test3_c1post (test3_cb fl))
@@ -265,7 +265,7 @@ let test3_ct_importable (fl:erased tflag) : safe_importable (test3_ct fl) fl tes
 [@@ (postprocess_with (fun () -> norm [delta_only [`%test3_ct; `%test3_cb;`%test3_ct_importable]]; trefl ()))]
 let test3 : src_interface = {
   mst = mst3;
-  pi = test3_pi; phi = test3_phi;
+  sgm = test3_sgm; pi = test3_pi;
   ct = test3_ct; ct_dcs = test3_rcs; ct_importable = test3_ct_importable; 
   psi = (fun _ _ _ -> True);
 }
@@ -285,5 +285,5 @@ let test3_ctx #fl sec_io eff_rcs fd =
   Inl (fun (fd:file_descr) -> Inl () <: (MIOwp (resexn unit) mst3 fl trivial_hist))
 
 val test3_ctx_t : ctx_tgt (comp_int_src_tgt test3)
-let test3_ctx_t #fl sec_io fd : MIOpi (resexn (file_descr -> MIOpi (resexn unit) fl test3_pi mst3)) fl test3_pi mst3 = 
-  Inl (fun (fd:file_descr) -> Inl () <: (MIOpi (resexn unit) fl test3_pi mst3))
+let test3_ctx_t #fl sec_io fd : MIOpi (resexn (file_descr -> MIOpi (resexn unit) fl test3_sgm mst3)) fl test3_sgm mst3 = 
+  Inl (fun (fd:file_descr) -> Inl () <: (MIOpi (resexn unit) fl test3_sgm mst3))
