io/case-studies/Compiler.Model2.Examples.fst
@@ -12,20 +12,20 @@ open Compiler.Model2
 type source_arrow (mst:mst) (arg:Type u#a) (res:Type u#b) (pre:arg -> trace -> Type0) (post:arg -> trace -> resexn res -> trace -> Type0) (fl:erased tflag) =
   x:arg -> MIO (resexn res) mst fl (pre x) (post x)
 
-type c1_post (#arg:Type u#a) (#res:Type u#b) (pre:arg -> trace -> Type0) (post:arg -> trace -> resexn res -> trace -> Type0) (pi:policy_spec) =
-  squash (forall x h lt. pre x h /\ enforced_locally pi h lt ==> post x h (Inr Contract_failure) lt)
+type c1_post (#arg:Type u#a) (#res:Type u#b) (pre:arg -> trace -> Type0) (post:arg -> trace -> resexn res -> trace -> Type0) (sgm:policy_spec) =
+  squash (forall x h lt. pre x h /\ enforced_locally sgm h lt ==> post x h (Inr Contract_failure) lt)
   
-type c2_post (#arg:Type u#a) (#res:Type u#b) (pre:arg -> trace -> Type0) (post:arg -> trace -> resexn res -> trace -> Type0) (pi:policy_spec) (#mst:mst) (dc:dc_typ mst #arg #(resexn res)) =
-  squash (forall x h r lt s0 s1. s0 `mst.models` h /\ s1 `mst.models` (apply_changes h lt) /\ pre x h /\ enforced_locally pi h lt /\ dc x s0 r s1 ==> post x h r lt)
+type c2_post (#arg:Type u#a) (#res:Type u#b) (pre:arg -> trace -> Type0) (post:arg -> trace -> resexn res -> trace -> Type0) (sgm:policy_spec) (#mst:mst) (dc:dc_typ mst #arg #(resexn res)) =
+  squash (forall x h r lt s0 s1. s0 `mst.models` h /\ s1 `mst.models` (apply_changes h lt) /\ pre x h /\ enforced_locally sgm h lt /\ dc x s0 r s1 ==> post x h r lt)
 
-type c1_pre (#arg:Type u#a) (#res:Type u#b) (pre:arg -> trace -> Type0) (post:arg -> trace -> resexn res -> trace -> Type0) (pi:policy_spec) (#mst:mst) (dc:dc_typ mst #arg #unit) =
+type c1_pre (#arg:Type u#a) (#res:Type u#b) (pre:arg -> trace -> Type0) (post:arg -> trace -> resexn res -> trace -> Type0) (sgm:policy_spec) (#mst:mst) (dc:dc_typ mst #arg #unit) =
   squash (forall x s0 s1 h. s0 `mst.models` h /\ s1 `mst.models` h /\ dc x s0 () s1 ==> pre x h)
 
-type c2_pre (#arg:Type u#a) (#res:Type u#b) (pre:arg -> trace -> Type0) (post:arg -> trace -> resexn res -> trace -> Type0) (pi:policy_spec) =
-  squash (forall x h lt r. pre x h /\ post x h r lt ==> enforced_locally pi h lt)
+type c2_pre (#arg:Type u#a) (#res:Type u#b) (pre:arg -> trace -> Type0) (post:arg -> trace -> resexn res -> trace -> Type0) (sgm:policy_spec) =
+  squash (forall x h lt r. pre x h /\ post x h r lt ==> enforced_locally sgm h lt)
 
-type stronger_pis (pi1:policy_spec) (pi2:policy_spec) =
-  squash (forall h lt. enforced_locally pi1 h lt ==> enforced_locally pi2 h lt)
+type stronger_sgms (sgm1:policy_spec) (sgm2:policy_spec) =
+  squash (forall h lt. enforced_locally sgm1 h lt ==> enforced_locally sgm2 h lt)
 
 let mst1 : mst = {
   cst = list file_descr;
@@ -34,14 +34,14 @@ let mst1 : mst = {
 
 (** ** Testing **)
 (** *** Test 1 - FO **)
-let test1_pi : policy_spec = 
+let test1_sgm : policy_spec = 
   fun h c cmd arg -> 
     Ctx? c /\
     (match cmd with 
     | Openfile -> (arg <> "/etc/passwd")
     | _ -> True)
 
-let test1_phi : policy mst1 test1_pi =
+let test1_pi : policy mst1 test1_sgm =
   fun h cmd arg -> 
     match cmd, arg with 
     | Openfile, s -> 
@@ -50,7 +50,7 @@ let test1_phi : policy mst1 test1_pi =
     | _ -> true
 
 let test1_pre = (fun (fd:file_descr) h -> b2t(is_open fd h))
-let test1_post = (fun (fd:file_descr) h (r:resexn unit) lt -> enforced_locally test1_pi h lt)
+let test1_post = (fun (fd:file_descr) h (r:resexn unit) lt -> enforced_locally test1_sgm h lt)
 
 type test1_pt = source_arrow mst1 file_descr unit test1_pre test1_post
     
@@ -60,13 +60,13 @@ let test1_pt_rcs : tree (pck_dc mst1) =
     Leaf 
     Leaf
 
-val test1_c1_pre : c1_pre test1_pre test1_post test1_pi test1_pt_rc
+val test1_c1_pre : c1_pre test1_pre test1_post test1_sgm test1_pt_rc
 let test1_c1_pre = ()
 
-val test1_c2_pre : c2_pre test1_pre test1_post test1_pi
+val test1_c2_pre : c2_pre test1_pre test1_post test1_sgm
 let test1_c2_pre = ()
 
-let test1_pt_exportable (fl:erased tflag) : exportable (test1_pt fl) fl test1_pi mst1 test1_pt_rcs =
+let test1_pt_exportable (fl:erased tflag) : exportable (test1_pt fl) fl test1_sgm mst1 test1_pt_rcs =
   exportable_arrow_pre_post_args
     _ _
     test1_pre
@@ -74,11 +74,11 @@ let test1_pt_exportable (fl:erased tflag) : exportable (test1_pt fl) fl test1_pi
     #test1_c1_pre
     #test1_c2_pre
                                                   
-val test1_stronger_pis : stronger_pis test1_pi test1_pi
-let test1_stronger_pis = 
+val test1_stronger_sgms : stronger_sgms test1_sgm test1_sgm
+let test1_stronger_sgms = 
   let rec aux (h:trace) (lt:trace) : Lemma
-    (requires (enforced_locally test1_pi h lt))
-    (ensures (enforced_locally test1_pi h lt))
+    (requires (enforced_locally test1_sgm h lt))
+    (ensures (enforced_locally test1_sgm h lt))
     (decreases lt) = (match lt with
     | [] -> ()
     | e :: tail -> aux (e::h) tail) in 
@@ -87,7 +87,7 @@ let test1_stronger_pis =
 [@@ (postprocess_with (fun () -> norm [delta_only [`%test1_pt; `%source_arrow; `%test1_pt_exportable]]; trefl ()))]
 let test1 : src_interface = {
   mst = mst1;
-  pi = test1_pi; phi = test1_phi;
+  sgm = test1_sgm; pi = test1_pi;
 
   pt = test1_pt;
   pt_dcs = test1_pt_rcs;
@@ -103,7 +103,7 @@ let test1_prog #fl fd : MIO (resexn unit) mst1 (fl+IOActions) (test1_pre fd) (te
   r <: resexn unit
 
 val test1_ctx : ctx_src test1
-let test1_ctx #fl io_acts eff_rcs prog () : MIOpi int fl test1.pi mst1 = 
+let test1_ctx #fl io_acts eff_rcs prog () : MIOpi int fl test1.sgm mst1 = 
   let fd = io_acts Openfile "/etc/passwd" in
   (match fd with
   | Inl fd -> let _ = prog fd in ()
@@ -111,7 +111,7 @@ let test1_ctx #fl io_acts eff_rcs prog () : MIOpi int fl test1.pi mst1 =
   0
 
 val test1_ctx_t : ctx_tgt (comp_int_src_tgt test1)
-let test1_ctx_t #fl io_acts prog () : MIOpi int fl test1.pi mst1 =
+let test1_ctx_t #fl io_acts prog () : MIOpi int fl test1.sgm mst1 =
   let fd = io_acts Openfile "/etc/passwd" in
   (match fd with
   | Inl fd -> let _ = prog fd in ()
