io/case-studies/IOLogging.fst
@@ -12,20 +12,20 @@ open Compiler.Model2
 type source_arrow (mst:mst) (arg:Type u#a) (res:Type u#b) (pre:arg -> trace -> Type0) (post:arg -> trace -> resexn res -> trace -> Type0) (fl:erased tflag) =
   x:arg -> MIO (resexn res) mst fl (pre x) (post x)
 
-type c1_post (#arg:Type u#a) (#res:Type u#b) (pre:arg -> trace -> Type0) (post:arg -> trace -> resexn res -> trace -> Type0) (pi:policy_spec) =
-  squash (forall x h lt. pre x h /\ enforced_locally pi h lt ==> post x h (Inr Contract_failure) lt)
+type c1_post (#arg:Type u#a) (#res:Type u#b) (pre:arg -> trace -> Type0) (post:arg -> trace -> resexn res -> trace -> Type0) (sgm:policy_spec) =
+  squash (forall x h lt. pre x h /\ enforced_locally sgm h lt ==> post x h (Inr Contract_failure) lt)
 
-type c2_post (#arg:Type u#a) (#res:Type u#b) (pre:arg -> trace -> Type0) (post:arg -> trace -> resexn res -> trace -> Type0) (pi:policy_spec) (#mst:mst) (dc:dc_typ mst #arg #(resexn res)) =
-  squash (forall x h r lt s0 s1. s0 `mst.models` h /\ s1 `mst.models` (apply_changes h lt) /\ pre x h /\ enforced_locally pi h lt /\ dc x s0 r s1 ==> post x h r lt)
+type c2_post (#arg:Type u#a) (#res:Type u#b) (pre:arg -> trace -> Type0) (post:arg -> trace -> resexn res -> trace -> Type0) (sgm:policy_spec) (#mst:mst) (dc:dc_typ mst #arg #(resexn res)) =
+  squash (forall x h r lt s0 s1. s0 `mst.models` h /\ s1 `mst.models` (apply_changes h lt) /\ pre x h /\ enforced_locally sgm h lt /\ dc x s0 r s1 ==> post x h r lt)
 
-type c1_pre (#arg:Type u#a) (#res:Type u#b) (pre:arg -> trace -> Type0) (post:arg -> trace -> resexn res -> trace -> Type0) (pi:policy_spec) (#mst:mst) (dc:dc_typ mst #arg #unit) =
+type c1_pre (#arg:Type u#a) (#res:Type u#b) (pre:arg -> trace -> Type0) (post:arg -> trace -> resexn res -> trace -> Type0) (sgm:policy_spec) (#mst:mst) (dc:dc_typ mst #arg #unit) =
   squash (forall x s0 s1 h. s0 `mst.models` h /\ s1 `mst.models` h /\ dc x s0 () s1 ==> pre x h)
 
-type c2_pre (#arg:Type u#a) (#res:Type u#b) (pre:arg -> trace -> Type0) (post:arg -> trace -> resexn res -> trace -> Type0) (pi:policy_spec) =
-  squash (forall x h lt r. pre x h /\ post x h r lt ==> enforced_locally pi h lt)
+type c2_pre (#arg:Type u#a) (#res:Type u#b) (pre:arg -> trace -> Type0) (post:arg -> trace -> resexn res -> trace -> Type0) (sgm:policy_spec) =
+  squash (forall x h lt r. pre x h /\ post x h r lt ==> enforced_locally sgm h lt)
 
-type stronger_pis (pi1:policy_spec) (pi2:policy_spec) =
-  squash (forall h lt. enforced_locally pi1 h lt ==> enforced_locally pi2 h lt)
+type stronger_sgms (sgm1:policy_spec) (sgm2:policy_spec) =
+  squash (forall h lt. enforced_locally sgm1 h lt ==> enforced_locally sgm2 h lt)
 
 
 
@@ -54,8 +54,8 @@ let to_string o =
   | Write -> "Write ..."
   | Close -> "Close ..."
 
-val pi : policy_spec
-let pi h c cmd arg =
+val sgm : policy_spec
+let sgm h c cmd arg =
   match c, cmd with
   | Ctx, _ ->
     h =!= []
@@ -66,16 +66,16 @@ let pi h c cmd arg =
     Nil? h \/ (get_caller (List.Tot.hd h) == Ctx)
   | _ -> False
 
-val phi0 : s:mymst.cst -> cmd:io_cmds -> arg:io_sig.args cmd -> r:bool
-let phi0 (s0:option event) cmd arg =
+val pi0 : s:mymst.cst -> cmd:io_cmds -> arg:io_sig.args cmd -> r:bool
+let pi0 (s0:option event) cmd arg =
   match s0 with
   | Some (EWrite Prog (fd, inp) (Inl ())) ->
     fd = stdout && inp = to_string cmd
   | _ -> false
 
-val phi : policy mymst pi
-let phi s0 cmd arg = 
-  phi0 s0 cmd arg
+val pi : policy mymst sgm
+let pi s0 cmd arg = 
+  pi0 s0 cmd arg
 
 let log_pre = (fun (op:io_cmds) (h:trace) -> h == [] \/ get_caller (List.Tot.hd h) == Ctx)
 let log_post = (fun (op:io_cmds) h (r:resexn unit) lt -> r =!= Inr Contract_failure /\ lt == [EWrite Prog (stdout, to_string op) r])
@@ -88,20 +88,20 @@ let log_pt_rcs : tree (pck_dc mymst) =
      Leaf
      Leaf
 
-val log_c1_pre : c1_pre log_pre log_post pi log_pt_rc
+val log_c1_pre : c1_pre log_pre log_post sgm log_pt_rc
 let log_c1_pre = ()
 
-val log_c2_pre : c2_pre log_pre log_post pi
+val log_c2_pre : c2_pre log_pre log_post sgm
 let log_c2_pre = ()
 
-instance interm_io_cmds fl pi mst : interm io_cmds fl pi mst = { mldummy = () }
-instance importable_io_cmds (#fl:erased tflag) (#pi:policy_spec) #mst : importable io_cmds fl pi mst Leaf = {
+instance interm_io_cmds fl sgm mst : interm io_cmds fl sgm mst = { mldummy = () }
+instance importable_io_cmds (#fl:erased tflag) (#sgm:policy_spec) #mst : importable io_cmds fl sgm mst Leaf = {
   ityp = io_cmds;
   c_ityp = solve;
   import = (fun x Leaf -> Inl x)
 }
 
-let log_pt_exportable (fl:erased tflag) : exportable (log_pt fl) fl pi mymst log_pt_rcs =
+let log_pt_exportable (fl:erased tflag) : exportable (log_pt fl) fl sgm mymst log_pt_rcs =
    exportable_arrow_pre_post_args
      _ _
      log_pre
@@ -109,11 +109,11 @@ let log_pt_exportable (fl:erased tflag) : exportable (log_pt fl) fl pi mymst log
      #log_c1_pre
      #log_c2_pre
 
-val log_stronger_pis : stronger_pis pi pi
-let log_stronger_pis =
+val log_stronger_sgms : stronger_sgms sgm sgm
+let log_stronger_sgms =
    let rec aux (h:trace) (lt:trace) : Lemma
-     (requires (enforced_locally pi h lt))
-     (ensures (enforced_locally pi h lt))
+     (requires (enforced_locally sgm h lt))
+     (ensures (enforced_locally sgm h lt))
      (decreases lt) = (match lt with
      | [] -> ()
      | e :: tail -> aux (e::h) tail) in
@@ -122,7 +122,7 @@ let log_stronger_pis =
 [@@ (postprocess_with (fun () -> norm [delta_only [`%log_pt; `%source_arrow; `%log_pt_exportable]]; trefl ()))]
  let test1 : src_interface = {
    mst = mymst;
-   pi = pi; phi = phi;
+   sgm = sgm; pi = pi;
 
    pt = log_pt;
    pt_dcs = log_pt_rcs;
@@ -137,15 +137,15 @@ let test1_prog #fl op : MIO (resexn unit) mymst (fl+IOActions) (log_pre op) (log
   let r : (mio_sig mymst).res Write (stdout, to_string op) = static_cmd Prog Write (stdout, to_string op) in
   r <: resexn unit
 
-assume val lemma_append_enforced_locally : pi:_ ->
+assume val lemma_append_enforced_locally : sgm:_ ->
   Lemma (forall h lt1 lt2.
-      enforced_locally pi h lt1 /\
-      enforced_locally pi (apply_changes h lt1) lt2 ==>
-      enforced_locally pi h (lt1 @ lt2))
+      enforced_locally sgm h lt1 /\
+      enforced_locally sgm (apply_changes h lt1) lt2 ==>
+      enforced_locally sgm h (lt1 @ lt2))
   
 val test1_ctx_t : ctx_tgt (comp_int_src_tgt test1)
-let test1_ctx_t #fl io_acts prog () : MIOpi int fl test1.pi mymst =
-  lemma_append_enforced_locally test1.pi;
+let test1_ctx_t #fl io_acts prog () : MIOpi int fl test1.sgm mymst =
+  lemma_append_enforced_locally test1.sgm;
   let _ = prog Openfile in
   let fd = io_acts Openfile "/etc/passwd" in
   0
