io/Compiler.ModelStlc.fst
@@ -20,22 +20,22 @@ let ctx_env =
           empty)
 
 #push-options "--compat_pre_core 1"
-let bt_ctx (e:exp{ELam? e}) (t:typ) (h:typing ctx_env e t) (#fl:erased tflag) (#pi:policy_spec) (#mst:mst) (sec_io:io_lib fl pi mst Ctx) : (typ_to_fstar t fl pi mst) =
-   let write : FStar.Universe.raise_t file_descr * FStar.Universe.raise_t string -> MIOpi (either (FStar.Universe.raise_t unit) (FStar.Universe.raise_t exn)) fl pi _ = fun fdb ->
+let bt_ctx (e:exp{ELam? e}) (t:typ) (h:typing ctx_env e t) (#fl:erased tflag) (#sgm:policy_spec) (#mst:mst) (sec_io:io_lib fl sgm mst Ctx) : (typ_to_fstar t fl sgm mst) =
+   let write : FStar.Universe.raise_t file_descr * FStar.Universe.raise_t string -> MIOpi (either (FStar.Universe.raise_t unit) (FStar.Universe.raise_t exn)) fl sgm _ = fun fdb ->
      let fd = FStar.Universe.downgrade_val (fst fdb) in
      let b = FStar.Universe.downgrade_val (snd fdb) in
      match sec_io Write (fd, b) with
      | Inl unit -> Inl (FStar.Universe.raise_val unit)
      | Inr ex -> Inr (FStar.Universe.raise_val ex) in
-   let openfile : FStar.Universe.raise_t string -> MIOpi (either (FStar.Universe.raise_t file_descr) (FStar.Universe.raise_t exn)) fl pi _ = fun s ->
+   let openfile : FStar.Universe.raise_t string -> MIOpi (either (FStar.Universe.raise_t file_descr) (FStar.Universe.raise_t exn)) fl sgm _ = fun s ->
      let s = FStar.Universe.downgrade_val s in
      match sec_io Openfile s with
      | Inl fd -> Inl (FStar.Universe.raise_val fd)
      | Inr ex -> Inr (FStar.Universe.raise_val ex) in
    let ctx_venv = 
-     vextend #fl #mst #pi #(TArr TString (TSum TFDesc TExn)) openfile (
-     vextend #fl #mst #pi #(TArr (TPair TFDesc TString) (TSum TUnit TExn)) write (
-     vempty #fl #pi #mst)) in
+     vextend #fl #mst #sgm #(TArr TString (TSum TFDesc TExn)) openfile (
+     vextend #fl #mst #sgm #(TArr (TPair TFDesc TString) (TSum TUnit TExn)) write (
+     vempty #fl #sgm #mst)) in
    exp_to_fstar' ctx_env e t h ctx_venv
 #pop-options
 
@@ -44,22 +44,22 @@ let bt_ctx (e:exp{ELam? e}) (t:typ) (h:typing ctx_env e t) (#fl:erased tflag) (#
 noeq
 type src_interface = {
   mst : mst;
-  (* pi is in Type0 and it is used at the level of the spec,
+  (* sgm is in Type0 and it is used at the level of the spec,
      it describes both the events done by the partial program and the context **)
-  pi : policy_spec;
-  (* phi is in bool and it is used to enfodce the policy on the context,
-     it describes only the events of the context and it has to imply pi **)
-  phi : policy mst pi;
+  sgm : policy_spec;
+  (* pi is in bool and it is used to enfodce the policy on the context,
+     it describes only the events of the context and it has to imply sgm **)
+  pi : policy mst sgm;
 
   (** The type of the "context" --- not sure if it is the best name.
       It is more like the type of the interface which the two share to communicate. **)
   ct : erased tflag -> Type;
   ct_dcs : tree (pck_dc mst);
-  ct_importable : fl:erased tflag -> safe_importable (ct fl) fl pi mst ct_dcs;
+  ct_importable : fl:erased tflag -> safe_importable (ct fl) fl sgm mst ct_dcs;
 
 
   wct : typ;
-  _c : fl:erased tflag -> Lemma ((ct_importable fl).ityp == (typ_to_fstar wct fl pi mst));
+  _c : fl:erased tflag -> Lemma ((ct_importable fl).ityp == (typ_to_fstar wct fl sgm mst));
 
   (** The partial program can have a post-condition that becomes the
       post-condition of the whole program after linking in the source.
@@ -70,19 +70,19 @@ type src_interface = {
 noeq
 type tgt_interface = {
   mst : mst;
-  pi : policy_spec;
-  phi : policy mst pi;
+  sgm : policy_spec;
+  pi : policy mst sgm;
 
   ct : typ;
 }
   
 (** **** languages **)
-type ctx_src (i:src_interface)  = #fl:erased tflag -> io_lib fl i.pi i.mst Ctx -> typ_eff_dcs i.mst fl i.ct_dcs -> i.ct fl 
+type ctx_src (i:src_interface)  = #fl:erased tflag -> io_lib fl i.sgm i.mst Ctx -> typ_eff_dcs i.mst fl i.ct_dcs -> i.ct fl 
 type prog_src (i:src_interface) = #fl:erased tflag -> i.ct (fl+IOActions) -> unit -> MIO int i.mst (IOActions + fl) (fun _ -> True) i.psi
 type whole_src = mst:mst & post:(trace -> int -> trace -> Type0) & (unit -> MIO int mst AllActions (fun _ -> True) post)
 
 let link_src (#i:src_interface) (p:prog_src i) (c:ctx_src i) : whole_src = 
-  (| i.mst, i.psi,  p #AllActions (c #AllActions (inst_io_cmds i.phi) (make_dcs_eff i.ct_dcs)) |)
+  (| i.mst, i.psi,  p #AllActions (c #AllActions (inst_io_cmds i.pi) (make_dcs_eff i.ct_dcs)) |)
 
 val beh_src : whole_src ^-> trace_property #event
 let beh_src = on_domain whole_src (fun (| mst, _, ws |) -> beh mst ws)
@@ -95,13 +95,13 @@ let src_language : language = {
 }
 
 type ctx_tgt (i:tgt_interface) = e:exp{ELam? e} & typing ctx_env e i.ct
-type prog_tgt (i:tgt_interface) = (typ_to_fstar i.ct AllActions i.pi i.mst) -> unit -> MIO int i.mst AllActions (fun _ -> True) (fun _ _ _ -> True)
+type prog_tgt (i:tgt_interface) = (typ_to_fstar i.ct AllActions i.sgm i.mst) -> unit -> MIO int i.mst AllActions (fun _ -> True) (fun _ _ _ -> True)
 type whole_tgt = mst:mst & (unit -> MIO int mst AllActions (fun _ -> True) (fun _ _ _ -> True))
 
 let link_tgt (#i:tgt_interface) (p:prog_tgt i) (c:ctx_tgt i) : whole_tgt =
   let (| e, h |) = c in
-  let sec_io = inst_io_cmds i.phi in
-  let c' = bt_ctx e i.ct h #AllActions #i.pi #i.mst sec_io in
+  let sec_io = inst_io_cmds i.pi in
+  let c' = bt_ctx e i.ct h #AllActions #i.sgm #i.mst sec_io in
   (| i.mst , p c' |)
 
 val beh_tgt : whole_tgt ^-> trace_property #event
@@ -119,19 +119,19 @@ let comp_int_src_tgt (i:src_interface) : tgt_interface = {
   ct = i.wct;
 
   mst = i.mst;
+  sgm = i.sgm;
   pi = i.pi;
-  phi = i.phi;
 }
 
 (** ** Compilation **)
-let convert (i:src_interface) fl (c:(typ_to_fstar i.wct fl i.pi i.mst)) : (i.ct_importable fl).ityp =
+let convert (i:src_interface) fl (c:(typ_to_fstar i.wct fl i.sgm i.mst)) : (i.ct_importable fl).ityp =
   i._c fl;
  c
 
 val backtranslate_ctx : (#i:src_interface) -> (c_t:ctx_tgt (comp_int_src_tgt i)) -> src_language.ctx i
 let backtranslate_ctx #i c_t #fl io_lib eff_dcs =
   let (| e, h |) = c_t in
-  let c' = bt_ctx e i.wct h #fl #i.pi #i.mst io_lib in
+  let c' = bt_ctx e i.wct h #fl #i.sgm #i.mst io_lib in
   (i.ct_importable fl).safe_import (convert i fl c') eff_dcs
 
 val compile_whole : whole_src -> whole_tgt
@@ -215,14 +215,14 @@ let wct = TArr TFDesc (TArr TBytes (TArr (TArr TBytes (TSum TUnit TExn)) (TSum T
 
 let test : src_interface = {
   mst = WS.cs_int.mst;
+  sgm = WS.cs_int.pi;
   pi = WS.cs_int.pi;
-  phi = WS.cs_int.phi;
   ct = WS.cs_int.ct;
   ct_dcs = WS.cs_int.ct_dcs;
   ct_importable = (fun fl -> WS.cs_int.ct_importable fl);
 
   wct = wct; // TODO: write the proper type here
-  _c = (fun fl -> assert ((WS.cs_int.ct_importable fl).ityp == (typ_to_fstar wct fl WS.cs_int.pi WS.cs_int.mst))); // universe problems);
+  _c = (fun fl -> assert ((WS.cs_int.ct_importable fl).ityp == (typ_to_fstar wct fl WS.cs_int.sgm WS.cs_int.mst))); // universe problems);
 
   psi = WS.cs_int.psi;
 }
